proof/invariant-abstract/AARCH64/ArchKernelInit_AI.thy
@@ -371,7 +371,7 @@ lemma invs_A:
    apply (clarsimp simp: valid_arch_state_def)
    apply (rule conjI)
     apply (clarsimp simp: valid_asid_table_def state_defs)
-   apply (simp add: valid_arch_state_def vmid_inv_def vmid_for_asid_2_def valid_vmid_table_def
+   apply (simp add: valid_arch_state_def vmid_inv_def valid_vmid_table_def
                     valid_global_tables_2_def valid_numlistregs_def cur_vcpu_2_def is_inv_def
                     state_defs obj_at_def a_type_def word_bits_def obind_def empty_pt_def)
   apply (rule conjI, clarsimp simp: valid_cur_fpu_def is_tcb_cur_fpu_def obj_at_def state_defs)
